some first attempt at scope extrusion...

pi.sig
@@ -1,13 +1,13 @@
--- Signature for System F
 
 -- the types
 chan : Type
 proc : Type
 
 
--- Res : (bind chan in proc) -> proc
+
 -- the constructors for proc
 Zero : proc  
 Par : proc -> proc -> proc 
 Rcv : chan -> (bind chan in proc) -> proc
 Send : chan -> chan -> proc -> proc
+Nu : (bind chan in proc) -> proc
