test/pi.sig
@@ -1,13 +1,13 @@
--- Signature for System F
 
 -- the types
 chan : Type
 proc : Type
 
+
+
 -- the constructors for proc
-Nil : proc 
-Bang : proc -> proc 
-Res : (bind chan in proc) -> proc
+Zero : proc  
 Par : proc -> proc -> proc 
-In : chan -> (bind chan in proc) -> proc
-Out : chan -> chan -> proc -> proc
+Rcv : chan -> (bind chan in proc) -> proc
+Send : chan -> chan -> proc -> proc
+Nu : (bind chan in proc) -> proc
