theories/Semantics.v
@@ -4,7 +4,12 @@ Require Import unscoped.
 Require Import core.
 Import ProcSyn.Core.
 Import unscoped.UnscopedNotations.
+Require Import Coq.Logic.FunctionalExtensionality.
 
+
+Print proc.
+Print chan. 
+ 
 (*Open Scope subst_scope.
 
 Locate ".:".
@@ -15,16 +20,71 @@ Definition bar (sigma : nat -> chan) (P:proc) := P  [sigma].
 *)
 
 
-(*   (proc, |)  commutative monoid up to conga *)
+
+(* the assumed setting  (Bi denotes a binder):
+            
+                _______ <-- current location
+ nu nu  (B1...Bn    i  )
+        
+*)
+Definition swap_aux n i := 
+ match i-n with
+ | 0 => var_chan (1+n)
+ | 1 => var_chan (0+n)
+ | _ => var_chan i
+ end.
+
+ 
+(*should initially called with n=0.
+n is the number of binder we have traversed 
+from "Nu Nu"
+up to the current point in the AST.
+*)
+Fixpoint swap n P := match P with
+ | Zero         => Zero 
+ | Par P Q      => Par (swap n P) (swap n Q)
+ | Nu P         => Nu (swap (n+1) P)
+ | Send (var_chan i) (var_chan j) P   =>
+     let x:= (swap_aux n i) in
+     let y:= (swap_aux n j) in 
+     Send x y (swap n P)
+ | Rcv (var_chan i) P    =>
+     let x:= (swap_aux n i) in  
+     Rcv x (swap (n+1) P)
+ end.
+
+
+ 
+Definition shift_pr (P:proc) := P [fun x => var_chan (x+1)].  
+Definition shiftn_pr n (P:proc) := P [fun x => var_chan (x+n)].  
+Definition shift_sub := fun x => var_chan (x+1).
+
 Inductive conga: proc -> proc -> Prop :=
 | Cga_parCom: forall P Q,     conga (Par P Q)  (Par Q P)
 | Cga_parAssoc: forall P Q R, conga (Par (Par P Q) R)    (Par P (Par Q R))
 | Cga_parNeut: forall P,      conga (Par P Zero) P
+(*
+| Cga_nuZero: conga (Nu Zero) Zero
+| Cga_nuPar: forall P Q,  conga (Par (Nu P) Q)   (Nu (Par P (shift_pr Q) ))
+| Cga_nuSwap: forall P, conga (Nu (Nu P))  (Nu (Nu (swap 0 P)))
+*).
+
+
+Inductive congb: proc -> proc -> Prop :=
+| Cgb_nuZero: congb (Nu Zero) Zero
+| Cgb_nuPar: forall P Q,  congb (Par (Nu P) Q)   (Nu (Par P (shift_pr Q) ))
+| Cgb_nuSwap: forall P, congb (Nu (Nu P))  (Nu (Nu (swap 0 P)))
 .
+
+
+
+
+
 
 (*  cong = conga + equivrel + ctxrules *)
 Inductive cong: proc -> proc -> Prop :=
 | Cg_cga: forall P Q,     conga P Q -> cong P Q
+| Cg_cgb: forall P Q,     congb P Q -> cong P Q
 | Cg_refl: forall P,       cong P P
 | Cg_sym: forall P Q,     cong Q P -> cong P Q
 | Cg_trans: forall P Q R, cong P Q -> cong Q R -> cong P R
@@ -32,18 +92,18 @@ Inductive cong: proc -> proc -> Prop :=
 | Cg_ctxParR: forall P Q Q', cong Q Q' -> cong (Par P Q) (Par P Q')
 | Cg_ctxSend: forall x y P P', cong P P' -> cong (Send x y P) (Send x y P')
 | Cg_ctxRcv: forall x P P', cong P P' -> cong (Rcv x P) (Rcv x P')
+| Cg_ctxNu: forall P Q,    cong P Q -> cong (Nu P) (Nu Q)
 .
 
-
+(* =====================INCOMPLET=========================================
+==============================================================*)
 
 Inductive lab :=
 | Lsend (x y: chan)
 | Lrcv (x y: chan)
+| LbdSend (x y: chan)
 | Ltau 
 .
-
-
-
 
 Inductive lt: proc -> lab -> proc -> Prop :=
 | Lt_send: forall x y P, lt (Send x y P) (Lsend x y) P 
@@ -55,6 +115,8 @@ Inductive lt: proc -> lab -> proc -> Prop :=
 | Lt_commR: forall P Q P' Q' x y, 
     lt P (Lrcv x y) P' -> lt Q (Lsend x y) Q' -> lt (Par P Q) Ltau (Par P' Q')
 .
+(*=============================================================
+==============================================================*)
 
 
 
@@ -62,17 +124,194 @@ Inductive red: proc -> proc -> Prop :=
 | Red_par: forall P Q R, red P Q -> red (Par P R) (Par Q R)
 | Red_struc: forall P P' Q Q',  cong P P' -> red P' Q' -> cong Q Q' -> red P Q
 | Red_comm: forall x y P P', red (Par (Send x y P) (Rcv x P')) (Par P (P' [y..]) )
+| Red_nu: forall P Q,    red P Q -> red (Nu P) (Nu Q)
 .
 
+(*
 
+        P --> Q
+  ----------------------
+    (nux) P --> (nux) Q
+
+*)
 
  
-Hint Constructors proc conga cong lab lt red: picalc. 
+Hint Constructors congb proc conga cong lab lt red: picalc. 
+
+
+Fixpoint iter_nu n P := match n with
+ | 0   => P
+ | S n => Nu (iter_nu n P)
+ end.
+
+
+Lemma iter_nu_cong: forall P Q R n,
+  cong P (iter_nu n Q) -> cong (Par P R) (Par (iter_nu n Q) R).  
+Proof.
+intros. 
+induction n; unfold iter_nu; eauto with picalc.
+Qed.
+
+
+
+Lemma conga_resp_sub: forall P Q sigma,
+  conga P Q -> conga (P [sigma]) (Q [sigma]).
+Proof.
+intros.
+inversion H; asimpl; eauto with picalc.
+Qed.
+
+
+Definition lift sigma := 
+ 0 .: (sigma >> S ).
+
+ 
+Lemma bind_simpl: forall sigma,
+ shift >> lift sigma = sigma >> shift .
+Proof.
+intro.
+symmetry.
+unfold funcomp. unfold lift.
+apply functional_extensionality.
+intro.
+unfold shift. unfold funcomp.
+cbv. auto.
+Qed.
+
+
+Lemma cong_resp_sub: forall P Q sigma,
+  cong P Q -> cong (P [sigma]) (Q [sigma]).
+Proof.
+intros. 
+generalize dependent sigma.  
+induction H; try(asimpl; eauto with picalc).
+intro.
+econstructor.
+eauto using conga_resp_sub.
+intro.
+
+inversion H; eauto with picalc. 
+subst.    
+eapply Cg_cgb.
+asimpl.
+
+
+rewrite bind_simpl.
+eapply Cgb_nuPar.
+eauto with picalc.
+
+
+
+eapply Cg_cgb.
+eauto with picalc.
+
+Qed.
+
+Hint Resolve cong_resp_sub: sublem.
+*)
+
+
+
+Lemma iden_ren: forall P:proc,  P [fun x => var_chan (x+0)] = P [fun x => var_chan (x)]. 
+Proof.
+intros.
+assert ((fun x : nat => (x + 0)__chan) = fun x : nat => x __chan).
+apply functional_extensionality.
+intros.
+auto.
+rewrite H.
+auto.
+Qed.
+
+(*
+Lemma iter_nu_scope_extr: forall n P Q,
+  cong (Par (iter_nu n P) Q)   (iter_nu n (Par P (shiftn_pr n Q) )).
+Proof.
+intros.
+induction n.
+unfold shiftn_pr. simpl.  
+rewrite iden_ren in *.
+asimpl. 
+eauto with picalc.
+
+simpl. 
+eapply Cg_ctxParL.
+eauto with picalc.
+*)
 
 
 
 
+Lemma red_normal: forall P Q ,
+  red P Q -> exists n S x y R1 R2 , 
+     cong P  (iter_nu n  (Par  (Par (Send x y R1) (Rcv x R2))    S) ) 
+     /\
+     cong Q  (iter_nu n  (Par (Par R1 (R2 [y..])  )   S)) .
+Proof.
+intros.
+induction H.   
+firstorder. 
+exists x. 
 
+
+(*
+generalize dependent x.
+intro. induction x.
+firstorder.
+simpl in *. 
+repeat eexists.
+eauto with picalc. eauto with picalc.
+firstorder. simpl in *.
+set (lem:= IHx H0 H1).
+*)
+
+
+repeat eexists.
+apply Cg_ctxParL with (Q:=R) in H0.
+induction x.  
+simpl in *. 
+eauto with picalc.
+simpl in *. 
+
+econstructor in  H0. eapply Cga_nuPar in H0. 
+
+
+
+eapply Cg_sym in .
+
+
+
+set (lem:= IHx  H1 H0).
+eauto with picalc.
+
+eapply Cg_ctxParL in H1.
+
+
+
+(*
+
+ P cong Nux1...Nuxn  (x0!x1.x2| x0?x3)|x 
+
+
+
+  P|R  cong   (x!y.R1| x?R2 )| S
+
+
+
+
+*)
+
+
+asimpl. 
+
+firstorder.
+exists 0. split.
+eauto with picalc.
+
+repeat eexists. 
+
+
+induction H;repeat eexists; eauto with picalc.
 
 
 
