theories/syntax/ProcSyn.v
@@ -133,26 +133,15 @@ exact (fun x => eq_refl).
 Qed.
 
 Inductive proc : Type :=
-  | Nil : proc
-  | Bang : proc -> proc
-  | Res : proc -> proc
+  | Zero : proc
   | Par : proc -> proc -> proc
-  | In : chan -> proc -> proc
-  | Out : chan -> chan -> proc -> proc.
+  | Rcv : chan -> proc -> proc
+  | Send : chan -> chan -> proc -> proc
+  | Nu : proc -> proc.
 
-Lemma congr_Nil : Nil = Nil.
+Lemma congr_Zero : Zero = Zero.
 Proof.
 exact (eq_refl).
-Qed.
-
-Lemma congr_Bang {s0 : proc} {t0 : proc} (H0 : s0 = t0) : Bang s0 = Bang t0.
-Proof.
-exact (eq_trans eq_refl (ap (fun x => Bang x) H0)).
-Qed.
-
-Lemma congr_Res {s0 : proc} {t0 : proc} (H0 : s0 = t0) : Res s0 = Res t0.
-Proof.
-exact (eq_trans eq_refl (ap (fun x => Res x) H0)).
 Qed.
 
 Lemma congr_Par {s0 : proc} {s1 : proc} {t0 : proc} {t1 : proc}
@@ -162,79 +151,82 @@ exact (eq_trans (eq_trans eq_refl (ap (fun x => Par x s1) H0))
          (ap (fun x => Par t0 x) H1)).
 Qed.
 
-Lemma congr_In {s0 : chan} {s1 : proc} {t0 : chan} {t1 : proc} (H0 : s0 = t0)
-  (H1 : s1 = t1) : In s0 s1 = In t0 t1.
+Lemma congr_Rcv {s0 : chan} {s1 : proc} {t0 : chan} {t1 : proc}
+  (H0 : s0 = t0) (H1 : s1 = t1) : Rcv s0 s1 = Rcv t0 t1.
 Proof.
-exact (eq_trans (eq_trans eq_refl (ap (fun x => In x s1) H0))
-         (ap (fun x => In t0 x) H1)).
+exact (eq_trans (eq_trans eq_refl (ap (fun x => Rcv x s1) H0))
+         (ap (fun x => Rcv t0 x) H1)).
 Qed.
 
-Lemma congr_Out {s0 : chan} {s1 : chan} {s2 : proc} {t0 : chan} {t1 : chan}
+Lemma congr_Send {s0 : chan} {s1 : chan} {s2 : proc} {t0 : chan} {t1 : chan}
   {t2 : proc} (H0 : s0 = t0) (H1 : s1 = t1) (H2 : s2 = t2) :
-  Out s0 s1 s2 = Out t0 t1 t2.
+  Send s0 s1 s2 = Send t0 t1 t2.
 Proof.
 exact (eq_trans
-         (eq_trans (eq_trans eq_refl (ap (fun x => Out x s1 s2) H0))
-            (ap (fun x => Out t0 x s2) H1))
-         (ap (fun x => Out t0 t1 x) H2)).
+         (eq_trans (eq_trans eq_refl (ap (fun x => Send x s1 s2) H0))
+            (ap (fun x => Send t0 x s2) H1))
+         (ap (fun x => Send t0 t1 x) H2)).
+Qed.
+
+Lemma congr_Nu {s0 : proc} {t0 : proc} (H0 : s0 = t0) : Nu s0 = Nu t0.
+Proof.
+exact (eq_trans eq_refl (ap (fun x => Nu x) H0)).
 Qed.
 
 Fixpoint subst_proc (sigma_chan : nat -> chan) (s : proc) {struct s} : 
 proc :=
   match s with
-  | Nil => Nil
-  | Bang s0 => Bang (subst_proc sigma_chan s0)
-  | Res s0 => Res (subst_proc (up_chan_chan sigma_chan) s0)
+  | Zero => Zero
   | Par s0 s1 => Par (subst_proc sigma_chan s0) (subst_proc sigma_chan s1)
-  | In s0 s1 =>
-      In (subst_chan sigma_chan s0) (subst_proc (up_chan_chan sigma_chan) s1)
-  | Out s0 s1 s2 =>
-      Out (subst_chan sigma_chan s0) (subst_chan sigma_chan s1)
+  | Rcv s0 s1 =>
+      Rcv (subst_chan sigma_chan s0)
+        (subst_proc (up_chan_chan sigma_chan) s1)
+  | Send s0 s1 s2 =>
+      Send (subst_chan sigma_chan s0) (subst_chan sigma_chan s1)
         (subst_proc sigma_chan s2)
+  | Nu s0 => Nu (subst_proc (up_chan_chan sigma_chan) s0)
   end.
 
 Fixpoint idSubst_proc (sigma_chan : nat -> chan)
 (Eq_chan : forall x, sigma_chan x = var_chan x) (s : proc) {struct s} :
 subst_proc sigma_chan s = s :=
   match s with
-  | Nil => congr_Nil
-  | Bang s0 => congr_Bang (idSubst_proc sigma_chan Eq_chan s0)
-  | Res s0 =>
-      congr_Res
-        (idSubst_proc (up_chan_chan sigma_chan) (upId_chan_chan _ Eq_chan) s0)
+  | Zero => congr_Zero
   | Par s0 s1 =>
       congr_Par (idSubst_proc sigma_chan Eq_chan s0)
         (idSubst_proc sigma_chan Eq_chan s1)
-  | In s0 s1 =>
-      congr_In (idSubst_chan sigma_chan Eq_chan s0)
+  | Rcv s0 s1 =>
+      congr_Rcv (idSubst_chan sigma_chan Eq_chan s0)
         (idSubst_proc (up_chan_chan sigma_chan) (upId_chan_chan _ Eq_chan) s1)
-  | Out s0 s1 s2 =>
-      congr_Out (idSubst_chan sigma_chan Eq_chan s0)
+  | Send s0 s1 s2 =>
+      congr_Send (idSubst_chan sigma_chan Eq_chan s0)
         (idSubst_chan sigma_chan Eq_chan s1)
         (idSubst_proc sigma_chan Eq_chan s2)
+  | Nu s0 =>
+      congr_Nu
+        (idSubst_proc (up_chan_chan sigma_chan) (upId_chan_chan _ Eq_chan) s0)
   end.
 
 Fixpoint ext_proc (sigma_chan : nat -> chan) (tau_chan : nat -> chan)
 (Eq_chan : forall x, sigma_chan x = tau_chan x) (s : proc) {struct s} :
 subst_proc sigma_chan s = subst_proc tau_chan s :=
   match s with
-  | Nil => congr_Nil
-  | Bang s0 => congr_Bang (ext_proc sigma_chan tau_chan Eq_chan s0)
-  | Res s0 =>
-      congr_Res
-        (ext_proc (up_chan_chan sigma_chan) (up_chan_chan tau_chan)
-           (upExt_chan_chan _ _ Eq_chan) s0)
+  | Zero => congr_Zero
   | Par s0 s1 =>
       congr_Par (ext_proc sigma_chan tau_chan Eq_chan s0)
         (ext_proc sigma_chan tau_chan Eq_chan s1)
-  | In s0 s1 =>
-      congr_In (ext_chan sigma_chan tau_chan Eq_chan s0)
+  | Rcv s0 s1 =>
+      congr_Rcv (ext_chan sigma_chan tau_chan Eq_chan s0)
         (ext_proc (up_chan_chan sigma_chan) (up_chan_chan tau_chan)
            (upExt_chan_chan _ _ Eq_chan) s1)
-  | Out s0 s1 s2 =>
-      congr_Out (ext_chan sigma_chan tau_chan Eq_chan s0)
+  | Send s0 s1 s2 =>
+      congr_Send (ext_chan sigma_chan tau_chan Eq_chan s0)
         (ext_chan sigma_chan tau_chan Eq_chan s1)
         (ext_proc sigma_chan tau_chan Eq_chan s2)
+  | Nu s0 =>
+      congr_Nu
+        (ext_proc (up_chan_chan sigma_chan) (up_chan_chan tau_chan)
+           (upExt_chan_chan _ _ Eq_chan) s0)
   end.
 
 Fixpoint compSubstSubst_proc (sigma_chan : nat -> chan)
@@ -244,30 +236,27 @@ Fixpoint compSubstSubst_proc (sigma_chan : nat -> chan)
 (s : proc) {struct s} :
 subst_proc tau_chan (subst_proc sigma_chan s) = subst_proc theta_chan s :=
   match s with
-  | Nil => congr_Nil
-  | Bang s0 =>
-      congr_Bang
-        (compSubstSubst_proc sigma_chan tau_chan theta_chan Eq_chan s0)
-  | Res s0 =>
-      congr_Res
-        (compSubstSubst_proc (up_chan_chan sigma_chan)
-           (up_chan_chan tau_chan) (up_chan_chan theta_chan)
-           (up_subst_subst_chan_chan _ _ _ Eq_chan) s0)
+  | Zero => congr_Zero
   | Par s0 s1 =>
       congr_Par
         (compSubstSubst_proc sigma_chan tau_chan theta_chan Eq_chan s0)
         (compSubstSubst_proc sigma_chan tau_chan theta_chan Eq_chan s1)
-  | In s0 s1 =>
-      congr_In
+  | Rcv s0 s1 =>
+      congr_Rcv
         (compSubstSubst_chan sigma_chan tau_chan theta_chan Eq_chan s0)
         (compSubstSubst_proc (up_chan_chan sigma_chan)
            (up_chan_chan tau_chan) (up_chan_chan theta_chan)
            (up_subst_subst_chan_chan _ _ _ Eq_chan) s1)
-  | Out s0 s1 s2 =>
-      congr_Out
+  | Send s0 s1 s2 =>
+      congr_Send
         (compSubstSubst_chan sigma_chan tau_chan theta_chan Eq_chan s0)
         (compSubstSubst_chan sigma_chan tau_chan theta_chan Eq_chan s1)
         (compSubstSubst_proc sigma_chan tau_chan theta_chan Eq_chan s2)
+  | Nu s0 =>
+      congr_Nu
+        (compSubstSubst_proc (up_chan_chan sigma_chan)
+           (up_chan_chan tau_chan) (up_chan_chan theta_chan)
+           (up_subst_subst_chan_chan _ _ _ Eq_chan) s0)
   end.
 
 Lemma substSubst_proc (sigma_chan : nat -> chan) (tau_chan : nat -> chan)
