test/syntax/ProcSyn.v
@@ -1,0 +1,532 @@
+Require Import core fintype.
+
+Require Import Setoid Morphisms Relation_Definitions.
+
+
+Module Core.
+
+Inductive chan (n_chan : nat) : Type :=
+    var_chan : fin n_chan -> chan n_chan.
+
+Definition subst_chan {m_chan : nat} {n_chan : nat}
+  (sigma_chan : fin m_chan -> chan n_chan) (s : chan m_chan) : chan n_chan :=
+  match s with
+  | var_chan _ s0 => sigma_chan s0
+  end.
+
+Lemma up_chan_chan {m : nat} {n_chan : nat} (sigma : fin m -> chan n_chan) :
+  fin (S m) -> chan (S n_chan).
+Proof.
+exact (scons (var_chan (S n_chan) var_zero)
+         (funcomp (subst_chan (funcomp (var_chan _) shift)) sigma)).
+Defined.
+
+Lemma up_list_chan_chan (p : nat) {m : nat} {n_chan : nat}
+  (sigma : fin m -> chan n_chan) : fin (plus p m) -> chan (plus p n_chan).
+Proof.
+exact (scons_p p (funcomp (var_chan (plus p n_chan)) (zero_p p))
+         (funcomp (subst_chan (funcomp (var_chan _) (shift_p p))) sigma)).
+Defined.
+
+Lemma upId_chan_chan {m_chan : nat} (sigma : fin m_chan -> chan m_chan)
+  (Eq : forall x, sigma x = var_chan m_chan x) :
+  forall x, up_chan_chan sigma x = var_chan (S m_chan) x.
+Proof.
+exact (fun n =>
+       match n with
+       | Some fin_n =>
+           ap (subst_chan (funcomp (var_chan _) shift)) (Eq fin_n)
+       | None => eq_refl
+       end).
+Qed.
+
+Lemma upId_list_chan_chan {p : nat} {m_chan : nat}
+  (sigma : fin m_chan -> chan m_chan)
+  (Eq : forall x, sigma x = var_chan m_chan x) :
+  forall x, up_list_chan_chan p sigma x = var_chan (plus p m_chan) x.
+Proof.
+exact (fun n =>
+       scons_p_eta (var_chan (plus p m_chan))
+         (fun n => ap (subst_chan (funcomp (var_chan _) (shift_p p))) (Eq n))
+         (fun n => eq_refl)).
+Qed.
+
+Definition idSubst_chan {m_chan : nat}
+  (sigma_chan : fin m_chan -> chan m_chan)
+  (Eq_chan : forall x, sigma_chan x = var_chan m_chan x) (s : chan m_chan) :
+  subst_chan sigma_chan s = s :=
+  match s with
+  | var_chan _ s0 => Eq_chan s0
+  end.
+
+Lemma upExt_chan_chan {m : nat} {n_chan : nat} (sigma : fin m -> chan n_chan)
+  (tau : fin m -> chan n_chan) (Eq : forall x, sigma x = tau x) :
+  forall x, up_chan_chan sigma x = up_chan_chan tau x.
+Proof.
+exact (fun n =>
+       match n with
+       | Some fin_n =>
+           ap (subst_chan (funcomp (var_chan _) shift)) (Eq fin_n)
+       | None => eq_refl
+       end).
+Qed.
+
+Lemma upExt_list_chan_chan {p : nat} {m : nat} {n_chan : nat}
+  (sigma : fin m -> chan n_chan) (tau : fin m -> chan n_chan)
+  (Eq : forall x, sigma x = tau x) :
+  forall x, up_list_chan_chan p sigma x = up_list_chan_chan p tau x.
+Proof.
+exact (fun n =>
+       scons_p_congr (fun n => eq_refl)
+         (fun n => ap (subst_chan (funcomp (var_chan _) (shift_p p))) (Eq n))).
+Qed.
+
+Definition ext_chan {m_chan : nat} {n_chan : nat}
+  (sigma_chan : fin m_chan -> chan n_chan)
+  (tau_chan : fin m_chan -> chan n_chan)
+  (Eq_chan : forall x, sigma_chan x = tau_chan x) (s : chan m_chan) :
+  subst_chan sigma_chan s = subst_chan tau_chan s :=
+  match s with
+  | var_chan _ s0 => Eq_chan s0
+  end.
+
+Definition compSubstSubst_chan {k_chan : nat} {l_chan : nat} {m_chan : nat}
+  (sigma_chan : fin m_chan -> chan k_chan)
+  (tau_chan : fin k_chan -> chan l_chan)
+  (theta_chan : fin m_chan -> chan l_chan)
+  (Eq_chan : forall x,
+             funcomp (subst_chan tau_chan) sigma_chan x = theta_chan x)
+  (s : chan m_chan) :
+  subst_chan tau_chan (subst_chan sigma_chan s) = subst_chan theta_chan s :=
+  match s with
+  | var_chan _ s0 => Eq_chan s0
+  end.
+
+Lemma up_subst_subst_chan_chan {k : nat} {l_chan : nat} {m_chan : nat}
+  (sigma : fin k -> chan l_chan) (tau_chan : fin l_chan -> chan m_chan)
+  (theta : fin k -> chan m_chan)
+  (Eq : forall x, funcomp (subst_chan tau_chan) sigma x = theta x) :
+  forall x,
+  funcomp (subst_chan (up_chan_chan tau_chan)) (up_chan_chan sigma) x =
+  up_chan_chan theta x.
+Proof.
+exact (fun n =>
+       match n with
+       | Some fin_n =>
+           eq_trans
+             (compSubstSubst_chan (funcomp (var_chan _) shift)
+                (up_chan_chan tau_chan)
+                (funcomp (up_chan_chan tau_chan) shift) (fun x => eq_refl)
+                (sigma fin_n))
+             (eq_trans
+                (eq_sym
+                   (compSubstSubst_chan tau_chan (funcomp (var_chan _) shift)
+                      (funcomp (subst_chan (funcomp (var_chan _) shift))
+                         tau_chan)
+                      (fun x => eq_refl) (sigma fin_n)))
+                (ap (subst_chan (funcomp (var_chan _) shift)) (Eq fin_n)))
+       | None => eq_refl
+       end).
+Qed.
+
+Lemma up_subst_subst_list_chan_chan {p : nat} {k : nat} {l_chan : nat}
+  {m_chan : nat} (sigma : fin k -> chan l_chan)
+  (tau_chan : fin l_chan -> chan m_chan) (theta : fin k -> chan m_chan)
+  (Eq : forall x, funcomp (subst_chan tau_chan) sigma x = theta x) :
+  forall x,
+  funcomp (subst_chan (up_list_chan_chan p tau_chan))
+    (up_list_chan_chan p sigma) x =
+  up_list_chan_chan p theta x.
+Proof.
+exact (fun n =>
+       eq_trans
+         (scons_p_comp' (funcomp (var_chan (plus p l_chan)) (zero_p p)) _ _ n)
+         (scons_p_congr
+            (fun x =>
+             scons_p_head' _
+               (fun z => subst_chan (funcomp (var_chan _) (shift_p p)) _) x)
+            (fun n =>
+             eq_trans
+               (compSubstSubst_chan (funcomp (var_chan _) (shift_p p))
+                  (up_list_chan_chan p tau_chan)
+                  (funcomp (up_list_chan_chan p tau_chan) (shift_p p))
+                  (fun x => eq_refl) (sigma n))
+               (eq_trans
+                  (eq_sym
+                     (compSubstSubst_chan tau_chan
+                        (funcomp (var_chan _) (shift_p p)) _
+                        (fun x => eq_sym (scons_p_tail' _ _ x)) (sigma n)))
+                  (ap (subst_chan (funcomp (var_chan _) (shift_p p))) (Eq n)))))).
+Qed.
+
+Lemma substSubst_chan {k_chan : nat} {l_chan : nat} {m_chan : nat}
+  (sigma_chan : fin m_chan -> chan k_chan)
+  (tau_chan : fin k_chan -> chan l_chan) (s : chan m_chan) :
+  subst_chan tau_chan (subst_chan sigma_chan s) =
+  subst_chan (funcomp (subst_chan tau_chan) sigma_chan) s.
+Proof.
+exact (compSubstSubst_chan sigma_chan tau_chan _ (fun n => eq_refl) s).
+Qed.
+
+Lemma substSubst_chan_pointwise {k_chan : nat} {l_chan : nat} {m_chan : nat}
+  (sigma_chan : fin m_chan -> chan k_chan)
+  (tau_chan : fin k_chan -> chan l_chan) :
+  pointwise_relation _ eq
+    (funcomp (subst_chan tau_chan) (subst_chan sigma_chan))
+    (subst_chan (funcomp (subst_chan tau_chan) sigma_chan)).
+Proof.
+exact (fun s =>
+       compSubstSubst_chan sigma_chan tau_chan _ (fun n => eq_refl) s).
+Qed.
+
+Lemma instId'_chan {m_chan : nat} (s : chan m_chan) :
+  subst_chan (var_chan m_chan) s = s.
+Proof.
+exact (idSubst_chan (var_chan m_chan) (fun n => eq_refl) s).
+Qed.
+
+Lemma instId'_chan_pointwise {m_chan : nat} :
+  pointwise_relation _ eq (subst_chan (var_chan m_chan)) id.
+Proof.
+exact (fun s => idSubst_chan (var_chan m_chan) (fun n => eq_refl) s).
+Qed.
+
+Lemma varL'_chan {m_chan : nat} {n_chan : nat}
+  (sigma_chan : fin m_chan -> chan n_chan) (x : fin m_chan) :
+  subst_chan sigma_chan (var_chan m_chan x) = sigma_chan x.
+Proof.
+exact (eq_refl).
+Qed.
+
+Lemma varL'_chan_pointwise {m_chan : nat} {n_chan : nat}
+  (sigma_chan : fin m_chan -> chan n_chan) :
+  pointwise_relation _ eq (funcomp (subst_chan sigma_chan) (var_chan m_chan))
+    sigma_chan.
+Proof.
+exact (fun x => eq_refl).
+Qed.
+
+Inductive proc (n_chan : nat) : Type :=
+  | Zero : proc n_chan
+  | Par : proc n_chan -> proc n_chan -> proc n_chan
+  | Rcv : chan n_chan -> proc (S n_chan) -> proc n_chan
+  | Send : chan n_chan -> chan n_chan -> proc n_chan -> proc n_chan
+  | Nu : proc (S n_chan) -> proc n_chan.
+
+Lemma congr_Zero {m_chan : nat} : Zero m_chan = Zero m_chan.
+Proof.
+exact (eq_refl).
+Qed.
+
+Lemma congr_Par {m_chan : nat} {s0 : proc m_chan} {s1 : proc m_chan}
+  {t0 : proc m_chan} {t1 : proc m_chan} (H0 : s0 = t0) (H1 : s1 = t1) :
+  Par m_chan s0 s1 = Par m_chan t0 t1.
+Proof.
+exact (eq_trans (eq_trans eq_refl (ap (fun x => Par m_chan x s1) H0))
+         (ap (fun x => Par m_chan t0 x) H1)).
+Qed.
+
+Lemma congr_Rcv {m_chan : nat} {s0 : chan m_chan} {s1 : proc (S m_chan)}
+  {t0 : chan m_chan} {t1 : proc (S m_chan)} (H0 : s0 = t0) (H1 : s1 = t1) :
+  Rcv m_chan s0 s1 = Rcv m_chan t0 t1.
+Proof.
+exact (eq_trans (eq_trans eq_refl (ap (fun x => Rcv m_chan x s1) H0))
+         (ap (fun x => Rcv m_chan t0 x) H1)).
+Qed.
+
+Lemma congr_Send {m_chan : nat} {s0 : chan m_chan} {s1 : chan m_chan}
+  {s2 : proc m_chan} {t0 : chan m_chan} {t1 : chan m_chan} {t2 : proc m_chan}
+  (H0 : s0 = t0) (H1 : s1 = t1) (H2 : s2 = t2) :
+  Send m_chan s0 s1 s2 = Send m_chan t0 t1 t2.
+Proof.
+exact (eq_trans
+         (eq_trans (eq_trans eq_refl (ap (fun x => Send m_chan x s1 s2) H0))
+            (ap (fun x => Send m_chan t0 x s2) H1))
+         (ap (fun x => Send m_chan t0 t1 x) H2)).
+Qed.
+
+Lemma congr_Nu {m_chan : nat} {s0 : proc (S m_chan)} {t0 : proc (S m_chan)}
+  (H0 : s0 = t0) : Nu m_chan s0 = Nu m_chan t0.
+Proof.
+exact (eq_trans eq_refl (ap (fun x => Nu m_chan x) H0)).
+Qed.
+
+Fixpoint subst_proc {m_chan : nat} {n_chan : nat}
+(sigma_chan : fin m_chan -> chan n_chan) (s : proc m_chan) {struct s} :
+proc n_chan :=
+  match s with
+  | Zero _ => Zero n_chan
+  | Par _ s0 s1 =>
+      Par n_chan (subst_proc sigma_chan s0) (subst_proc sigma_chan s1)
+  | Rcv _ s0 s1 =>
+      Rcv n_chan (subst_chan sigma_chan s0)
+        (subst_proc (up_chan_chan sigma_chan) s1)
+  | Send _ s0 s1 s2 =>
+      Send n_chan (subst_chan sigma_chan s0) (subst_chan sigma_chan s1)
+        (subst_proc sigma_chan s2)
+  | Nu _ s0 => Nu n_chan (subst_proc (up_chan_chan sigma_chan) s0)
+  end.
+
+Fixpoint idSubst_proc {m_chan : nat} (sigma_chan : fin m_chan -> chan m_chan)
+(Eq_chan : forall x, sigma_chan x = var_chan m_chan x) (s : proc m_chan)
+{struct s} : subst_proc sigma_chan s = s :=
+  match s with
+  | Zero _ => congr_Zero
+  | Par _ s0 s1 =>
+      congr_Par (idSubst_proc sigma_chan Eq_chan s0)
+        (idSubst_proc sigma_chan Eq_chan s1)
+  | Rcv _ s0 s1 =>
+      congr_Rcv (idSubst_chan sigma_chan Eq_chan s0)
+        (idSubst_proc (up_chan_chan sigma_chan) (upId_chan_chan _ Eq_chan) s1)
+  | Send _ s0 s1 s2 =>
+      congr_Send (idSubst_chan sigma_chan Eq_chan s0)
+        (idSubst_chan sigma_chan Eq_chan s1)
+        (idSubst_proc sigma_chan Eq_chan s2)
+  | Nu _ s0 =>
+      congr_Nu
+        (idSubst_proc (up_chan_chan sigma_chan) (upId_chan_chan _ Eq_chan) s0)
+  end.
+
+Fixpoint ext_proc {m_chan : nat} {n_chan : nat}
+(sigma_chan : fin m_chan -> chan n_chan)
+(tau_chan : fin m_chan -> chan n_chan)
+(Eq_chan : forall x, sigma_chan x = tau_chan x) (s : proc m_chan) {struct s}
+   :
+subst_proc sigma_chan s = subst_proc tau_chan s :=
+  match s with
+  | Zero _ => congr_Zero
+  | Par _ s0 s1 =>
+      congr_Par (ext_proc sigma_chan tau_chan Eq_chan s0)
+        (ext_proc sigma_chan tau_chan Eq_chan s1)
+  | Rcv _ s0 s1 =>
+      congr_Rcv (ext_chan sigma_chan tau_chan Eq_chan s0)
+        (ext_proc (up_chan_chan sigma_chan) (up_chan_chan tau_chan)
+           (upExt_chan_chan _ _ Eq_chan) s1)
+  | Send _ s0 s1 s2 =>
+      congr_Send (ext_chan sigma_chan tau_chan Eq_chan s0)
+        (ext_chan sigma_chan tau_chan Eq_chan s1)
+        (ext_proc sigma_chan tau_chan Eq_chan s2)
+  | Nu _ s0 =>
+      congr_Nu
+        (ext_proc (up_chan_chan sigma_chan) (up_chan_chan tau_chan)
+           (upExt_chan_chan _ _ Eq_chan) s0)
+  end.
+
+Fixpoint compSubstSubst_proc {k_chan : nat} {l_chan : nat} {m_chan : nat}
+(sigma_chan : fin m_chan -> chan k_chan)
+(tau_chan : fin k_chan -> chan l_chan)
+(theta_chan : fin m_chan -> chan l_chan)
+(Eq_chan : forall x,
+           funcomp (subst_chan tau_chan) sigma_chan x = theta_chan x)
+(s : proc m_chan) {struct s} :
+subst_proc tau_chan (subst_proc sigma_chan s) = subst_proc theta_chan s :=
+  match s with
+  | Zero _ => congr_Zero
+  | Par _ s0 s1 =>
+      congr_Par
+        (compSubstSubst_proc sigma_chan tau_chan theta_chan Eq_chan s0)
+        (compSubstSubst_proc sigma_chan tau_chan theta_chan Eq_chan s1)
+  | Rcv _ s0 s1 =>
+      congr_Rcv
+        (compSubstSubst_chan sigma_chan tau_chan theta_chan Eq_chan s0)
+        (compSubstSubst_proc (up_chan_chan sigma_chan)
+           (up_chan_chan tau_chan) (up_chan_chan theta_chan)
+           (up_subst_subst_chan_chan _ _ _ Eq_chan) s1)
+  | Send _ s0 s1 s2 =>
+      congr_Send
+        (compSubstSubst_chan sigma_chan tau_chan theta_chan Eq_chan s0)
+        (compSubstSubst_chan sigma_chan tau_chan theta_chan Eq_chan s1)
+        (compSubstSubst_proc sigma_chan tau_chan theta_chan Eq_chan s2)
+  | Nu _ s0 =>
+      congr_Nu
+        (compSubstSubst_proc (up_chan_chan sigma_chan)
+           (up_chan_chan tau_chan) (up_chan_chan theta_chan)
+           (up_subst_subst_chan_chan _ _ _ Eq_chan) s0)
+  end.
+
+Lemma substSubst_proc {k_chan : nat} {l_chan : nat} {m_chan : nat}
+  (sigma_chan : fin m_chan -> chan k_chan)
+  (tau_chan : fin k_chan -> chan l_chan) (s : proc m_chan) :
+  subst_proc tau_chan (subst_proc sigma_chan s) =
+  subst_proc (funcomp (subst_chan tau_chan) sigma_chan) s.
+Proof.
+exact (compSubstSubst_proc sigma_chan tau_chan _ (fun n => eq_refl) s).
+Qed.
+
+Lemma substSubst_proc_pointwise {k_chan : nat} {l_chan : nat} {m_chan : nat}
+  (sigma_chan : fin m_chan -> chan k_chan)
+  (tau_chan : fin k_chan -> chan l_chan) :
+  pointwise_relation _ eq
+    (funcomp (subst_proc tau_chan) (subst_proc sigma_chan))
+    (subst_proc (funcomp (subst_chan tau_chan) sigma_chan)).
+Proof.
+exact (fun s =>
+       compSubstSubst_proc sigma_chan tau_chan _ (fun n => eq_refl) s).
+Qed.
+
+Lemma instId'_proc {m_chan : nat} (s : proc m_chan) :
+  subst_proc (var_chan m_chan) s = s.
+Proof.
+exact (idSubst_proc (var_chan m_chan) (fun n => eq_refl) s).
+Qed.
+
+Lemma instId'_proc_pointwise {m_chan : nat} :
+  pointwise_relation _ eq (subst_proc (var_chan m_chan)) id.
+Proof.
+exact (fun s => idSubst_proc (var_chan m_chan) (fun n => eq_refl) s).
+Qed.
+
+Class Up_proc X Y :=
+    up_proc : X -> Y.
+
+Class Up_chan X Y :=
+    up_chan : X -> Y.
+
+#[global]
+Instance Subst_proc  {m_chan n_chan : nat}: (Subst1 _ _ _) :=
+ (@subst_proc m_chan n_chan).
+
+#[global]
+Instance Up_chan_chan  {m n_chan : nat}: (Up_chan _ _) :=
+ (@up_chan_chan m n_chan).
+
+#[global]
+Instance Subst_chan  {m_chan n_chan : nat}: (Subst1 _ _ _) :=
+ (@subst_chan m_chan n_chan).
+
+#[global]
+Instance VarInstance_chan  {n_chan : nat}: (Var _ _) := (@var_chan n_chan).
+
+Notation "s [ sigma_chan ]" := (subst_proc sigma_chan s)
+( at level 7, left associativity, only printing)  : subst_scope.
+
+Notation "↑__proc" := up_proc (only printing)  : subst_scope.
+
+Notation "↑__chan" := up_chan_chan (only printing)  : subst_scope.
+
+Notation "s [ sigma_chan ]" := (subst_chan sigma_chan s)
+( at level 7, left associativity, only printing)  : subst_scope.
+
+Notation "↑__chan" := up_chan (only printing)  : subst_scope.
+
+Notation "'var'" := var_chan ( at level 1, only printing)  : subst_scope.
+
+Notation "x '__chan'" := (@ids _ _ VarInstance_chan x)
+( at level 5, format "x __chan", only printing)  : subst_scope.
+
+Notation "x '__chan'" := (var_chan x) ( at level 5, format "x __chan")  :
+subst_scope.
+
+#[global]
+Instance subst_proc_morphism  {m_chan : nat} {n_chan : nat}:
+ (Proper (respectful (pointwise_relation _ eq) (respectful eq eq))
+    (@subst_proc m_chan n_chan)).
+Proof.
+exact (fun f_chan g_chan Eq_chan s t Eq_st =>
+       eq_ind s (fun t' => subst_proc f_chan s = subst_proc g_chan t')
+         (ext_proc f_chan g_chan Eq_chan s) t Eq_st).
+Qed.
+
+#[global]
+Instance subst_proc_morphism2  {m_chan : nat} {n_chan : nat}:
+ (Proper (respectful (pointwise_relation _ eq) (pointwise_relation _ eq))
+    (@subst_proc m_chan n_chan)).
+Proof.
+exact (fun f_chan g_chan Eq_chan s => ext_proc f_chan g_chan Eq_chan s).
+Qed.
+
+#[global]
+Instance subst_chan_morphism  {m_chan : nat} {n_chan : nat}:
+ (Proper (respectful (pointwise_relation _ eq) (respectful eq eq))
+    (@subst_chan m_chan n_chan)).
+Proof.
+exact (fun f_chan g_chan Eq_chan s t Eq_st =>
+       eq_ind s (fun t' => subst_chan f_chan s = subst_chan g_chan t')
+         (ext_chan f_chan g_chan Eq_chan s) t Eq_st).
+Qed.
+
+#[global]
+Instance subst_chan_morphism2  {m_chan : nat} {n_chan : nat}:
+ (Proper (respectful (pointwise_relation _ eq) (pointwise_relation _ eq))
+    (@subst_chan m_chan n_chan)).
+Proof.
+exact (fun f_chan g_chan Eq_chan s => ext_chan f_chan g_chan Eq_chan s).
+Qed.
+
+Ltac auto_unfold := repeat
+                     unfold VarInstance_chan, Var, ids, Subst_chan, Subst1,
+                      subst1, Up_chan_chan, Up_chan, up_chan, Subst_proc,
+                      Subst1, subst1.
+
+Tactic Notation "auto_unfold" "in" "*" := repeat
+                                           unfold VarInstance_chan, Var, ids,
+                                            Subst_chan, Subst1, subst1,
+                                            Up_chan_chan, Up_chan, up_chan,
+                                            Subst_proc, Subst1, subst1 
+                                            in *.
+
+Ltac asimpl' := repeat (first
+                 [ progress setoid_rewrite substSubst_proc_pointwise
+                 | progress setoid_rewrite substSubst_proc
+                 | progress setoid_rewrite substSubst_chan_pointwise
+                 | progress setoid_rewrite substSubst_chan
+                 | progress setoid_rewrite instId'_proc_pointwise
+                 | progress setoid_rewrite instId'_proc
+                 | progress setoid_rewrite varL'_chan_pointwise
+                 | progress setoid_rewrite varL'_chan
+                 | progress setoid_rewrite instId'_chan_pointwise
+                 | progress setoid_rewrite instId'_chan
+                 | progress unfold up_list_chan_chan, up_chan_chan, up_ren
+                 | progress cbn[subst_proc subst_chan]
+                 | progress fsimpl ]).
+
+Ltac asimpl := check_no_evars;
+                repeat
+                 unfold VarInstance_chan, Var, ids, Subst_chan, Subst1,
+                  subst1, Up_chan_chan, Up_chan, up_chan, Subst_proc, Subst1,
+                  subst1 in *;
+                asimpl'; minimize.
+
+Tactic Notation "asimpl" "in" hyp(J) := revert J; asimpl; intros J.
+
+Tactic Notation "auto_case" := auto_case ltac:(asimpl; cbn; eauto).
+
+Ltac substify := auto_unfold.
+
+Ltac renamify := auto_unfold.
+
+End Core.
+
+Module Extra.
+
+Import
+Core.
+
+Arguments Nu {n_chan}.
+
+Arguments Send {n_chan}.
+
+Arguments Rcv {n_chan}.
+
+Arguments Par {n_chan}.
+
+Arguments Zero {n_chan}.
+
+Arguments var_chan {n_chan}.
+
+#[global] Hint Opaque subst_proc: rewrite.
+
+#[global] Hint Opaque subst_chan: rewrite.
+
+End Extra.
+
+Module interface.
+
+Export Core.
+
+Export Extra.
+
+End interface.
+
+Export interface.
+
